veric/juicy_extspec.v
@@ -286,7 +286,7 @@ Proof.
           generalize (approx'_oo_approx (level m') (level jm)); intros H10.
           spec H10; [omega |].
           do 2 rewrite <-level_juice_level_phi.
-          rewrite MixVariantFunctorLemmas.fmap_app.
+          rewrite fmap_app.
           rewrite H9, H10; auto.
        ++ rewrite <-resource_at_approx, Hphi; auto.
       * intros adr. case_eq (m_phi m' @ adr); auto. intros k p Hm'.
